working on the unionfind example

examples/dm4free/Relational.UnionFind.fst
@@ -4,51 +4,45 @@ open FStar.Seq
 open FStar.DM4F.Heap
 open FStar.DM4F.Heap.ST
 
-(* immediate parent index, height (a.k.a. rank) of the node *)
-type elt = nat * nat
+type id (n:nat) = i:nat{i < n}
 
-(* array representation, ith index is the ith node maintaining its parent and height *)
-type uf_forest = seq (ref elt)
+type elt (n:nat) = id n * id n
 
-(* valid index in the union-find forest *)
-type id (uf:uf_forest) = i:nat{i < length uf}
+type uf_forest (n:nat) = s:seq (ref (elt n)){length s = n}
 
 (* liveness and separation condition for the forest *)
-let live (uf:uf_forest) (h:heap) :Type0 =
-  (forall (i:id uf).{:pattern addr_of (index uf i)} forall (j:id uf).{:pattern addr_of (index uf j)}
+let live (#n:nat) (uf:uf_forest n) (h:heap) :Type0 =
+  (forall (i:id n).{:pattern addr_of (index uf i)} forall (j:id n).{:pattern addr_of (index uf j)}
                i <> j ==> addr_of (index uf i) <> addr_of (index uf j)) /\  //all the refs in the forest are distinct
-  (forall (i:id uf).{:pattern (h `contains_a_well_typed` (index uf i))}
+  (forall (i:id n).{:pattern (h `contains_a_well_typed` (index uf i))}
                h `contains_a_well_typed` (index uf i))  //all the refs in the forest are well typed
 
 (* helpers for getting the parent and height *)
-unfold let parent (uf:uf_forest) (i:id uf) (h:heap) :GTot nat = fst (sel h (index uf i))
-unfold let height (uf:uf_forest) (i:id uf) (h:heap) :GTot nat = snd (sel h (index uf i))
+unfold let parent (#n:nat) (uf:uf_forest n) (i:id n) (h:heap) :GTot (id n) = fst (sel h (index uf i))
+unfold let height (#n:nat) (uf:uf_forest n) (i:id n) (h:heap) :GTot (id n) = snd (sel h (index uf i))
 
 (*
  * well-formed conditions on the forest, essentially the invariants needed for proving the termination of operations
  * TODO: add the pattern, perhaps {:pattern (sel h (index uf i))}?
  *)
-let well_formed (uf:uf_forest) (h:heap) =
-  forall (i:id uf).
-               parent uf i h < length uf /\
-               height uf i h < length uf /\
-               (parent uf i h = i \/ height uf i h < height uf (parent uf i h) h)
+let well_formed (#n:nat) (uf:uf_forest n) (h:heap) =
+  forall (i:id n).{:pattern (sel h (index uf i))}
+             (parent uf i h = i \/ height uf i h < height uf (parent uf i h) h)
 
 (*
  * the postcondition parent uf r h1 = r is added because of merge, see below in comments
  *)
-reifiable let rec find (uf:uf_forest) (i:id uf) (ghost_heap:heap)
-  :ST (id uf) (requires  (fun h0      -> ghost_heap == h0 /\ live uf h0 /\ well_formed uf h0))
+reifiable let rec find (#n:nat) (uf:uf_forest n) (i:id n) (ghost_heap:heap)
+  :ST (id n) (requires  (fun h0      -> ghost_heap == h0 /\ live uf h0 /\ well_formed uf h0))
               (ensures   (fun h0 r h1 -> h0 == h1 /\ parent uf r h1 = r))
-	      (decreases (length uf - height uf i ghost_heap))
+	      (decreases (length uf - height #n uf i ghost_heap))
   = let (p, _) = read (index uf i) in
     if p = i then i
     else begin
-      assert (forall (i:id uf). height uf i ghost_heap < length uf);  //this is an annoying assert, should go away with better modeling
       find uf p ghost_heap
     end      
 
-reifiable let rec merge (uf:uf_forest) (i_1:id uf) (i_2:id uf)
+reifiable let rec merge (#n:nat) (uf:uf_forest n) (i_1:id n) (i_2:id n)
   : ST unit (requires (fun h0      -> live uf h0 /\ well_formed uf h0))
             (ensures  (fun h0 _ h1 -> live uf h1 /\ well_formed uf h1))
   = let h0 = STATE?.get () in
@@ -74,15 +68,15 @@ reifiable let rec merge (uf:uf_forest) (i_1:id uf) (i_2:id uf)
         write ref_2 (r_2, d_1 + 1)
     end
 
-reifiable let rec find_opt (uf:uf_forest) (i:id uf) (ghost_heap:heap)
-  :ST (id uf) (requires (fun h0      -> ghost_heap == h0 /\ live uf h0 /\ well_formed uf h0))
-              (ensures  (fun h0 r h1 -> live uf h1 /\ well_formed uf h1 /\ parent uf r h1 = r /\  //these are from find
-	                             (r = i \/ height uf r h1 > height uf i h1) /\  //we need this because when we write p' as i's parent
+reifiable let rec find_opt (#n:nat) (uf:uf_forest n) (i:id n) (ghost_heap:heap)
+  :ST (id n) (requires (fun h0      -> ghost_heap == h0 /\ live uf h0 /\ well_formed uf h0))
+             (ensures  (fun h0 r h1 -> live uf h1 /\ well_formed uf h1 /\ parent uf r h1 = r /\  //these are from find
+	                            (r = i \/ height uf r h1 > height uf i h1) /\  //we need this because when we write p' as i's parent
 				                                                   //we need to ensure wellformedness i.e. height of p'
 										   //is more than the height of i
-				     (forall (j:id uf). height uf j h0 < height uf i h0 ==>
-	                                           sel h1 (index uf j) = sel h0 (index uf j))))  //this last clause to say that i remains unchanged in the recursive call, else when we write its height to be d, we have trouble proving that p's height is more than d
-	      (decreases (length uf - height uf i ghost_heap))
+				     (forall (j:id n).{:pattern (sel h1 (index uf j))} height uf j h0 < height uf i h0 ==>
+	                                          sel h1 (index uf j) = sel h0 (index uf j))))  //this last clause to say that i remains unchanged in the recursive call, else when we write its height to be d, we have trouble proving that p's height is more than d
+	      (decreases (length uf - height #n uf i ghost_heap))
   = let (p, d) = read (index uf i) in
     if p = i then i
     else
@@ -91,131 +85,130 @@ reifiable let rec find_opt (uf:uf_forest) (i:id uf) (ghost_heap:heap)
       write (index uf i) (p', d);
       p'
 
-let rec lemma_0 (uf:uf_forest) (i:id uf) (h:heap{live uf h /\ well_formed uf h})
-  :Lemma (requires  True)
-         (ensures   (let r0, h0 = reify (find uf i h) h in
-                     let r1, h1 = reify (find_opt uf i h) h in
-	             r0 = r1))
-	 (decreases (length uf - height uf i h))
-  = let p, _ = sel h (index uf i) in
+#set-options "--z3rlimit 50"
+let lemma_find_helper (#n:nat) (uf:uf_forest n) (i:id n) (h:heap{live uf h /\ well_formed uf h})
+  :Lemma (let p, d = sel h (index uf i) in
+          reify (find uf p h) h == reify (find uf i h) h)
+  = let p, s = sel h (index uf i) in
     if p = i then ()
-    else begin
-      assert (forall (i:id uf). height uf i h < length uf);
-      lemma_0 uf p h
-    end
+    else ()
+#reset-options
 
 #set-options "--z3rlimit 50"
-let rec lemma_1 (uf:uf_forest) (i:id uf) (h:heap{live uf h /\ well_formed uf h}) (j:id uf)
-  :Lemma (requires True)
-         (ensures  (let _, h0 = reify (find uf i h) h in
-	            let _, h1 = reify (find_opt uf i h) h in
+let lemma_find_opt_helper (#n:nat) (uf:uf_forest n) (i:id n) (h:heap{live uf h /\ well_formed uf h})
+  :Lemma (let p, d = sel h (index uf i) in
+          p = i \/
+	  (let pp, hp = reify (find_opt uf p h) h in
+            let pi, hi = reify (find_opt uf i h) h in
+	    pp = pi /\ (hi == upd hp (index uf i) (pp, d))))
+  = let p, s = sel h (index uf i) in
+    if p = i then ()
+    else ()
+#reset-options
 
-                    let p0, _ = sel h0 (index uf j) in
-		    let p1, _ = sel h1 (index uf j) in
+(* let lemma_0 (uf:uf_forest) (i:id uf) (h:heap{live uf h /\ well_formed uf h}) :GTot unit = *)
+(*   let p, s = sel h (index uf i) in *)
+(*   if p = i then () *)
+(*   else begin *)
+(*     let pp, h1 = reify (find_opt uf p h) h in *)
+(*     let _, h2 = reify (find_opt uf i h) h in *)
+(*     assert (h2 == upd h1 (index uf i) (pp, s)); *)
+(*     () *)
+(*   end *)
 
-                    p0 = p1 \/ (p1 = fst (reify (find uf j h0) h0) /\ parent uf p1 h1 = p1)))
-	 (decreases (length uf - height uf i h))
+(* let lemma_1 (uf:uf_forest) (i:id uf) (h:heap{live uf h /\ well_formed uf h}) :GTot unit = *)
+(*   let p, s = sel h (index uf i) in *)
+(*   if p = i then () *)
+(*   else begin *)
+(*     let pp, h1 = reify (find_opt uf p h) h in *)
+(*     let _, h2 = reify (find_opt uf i h) h in *)
+(*     assert (forall (a:Type) (r:ref a). addr_of r <> addr_of (index uf i) ==> sel h1 r == sel h2 r); *)
+(*     //assert (h2 == upd h1 (index uf i) (pp, s)); *)
+(*     () *)
+(*   end *)
+(*
+ * a simple warm up lemma
+ * proving that find and find_opt return the same value
+ * we don't prove anything about the resultant heaps, yet
+ *)
+let rec lemma_find_find_opt_same_result (#n:nat) (uf:uf_forest n) (i:id n) (h:heap{live uf h /\ well_formed uf h})
+  :Lemma (requires  True)
+         (ensures   (fst (reify (find uf i h) h) = fst (reify (find_opt uf i h) h)))
+	 (decreases (length uf - height #n uf i h))
   = let p, _ = sel h (index uf i) in
     if p = i then ()
     else begin
-      assert (forall (i:id uf). height uf i h < length uf);
-      lemma_1 uf p h j;
-      let _, h0 = reify (find uf p h) h in
-      let _, h1 = reify (find_opt uf p h) h in
-      let p0, _ = sel h0 (index uf j) in
-      let p1, _ = sel h1 (index uf j) in
-      assert (p0 = p1 \/ (p1 = fst (reify (find uf j h0) h0)));
-      lemma_0 uf i h;  //proof takes more time without this, since it has to unfold reify (find uf i h0) when j = i
-      lemma_0 uf p h
+      lemma_find_find_opt_same_result uf p h
     end
 
-let rec lemma_2 (uf:uf_forest) (i:id uf) (h:heap{live uf h /\ well_formed uf h}) (j:id uf)
+(*
+ * after find_opt, either parent of a node j remains same, or
+ * the parent is j's root in the original heap
+ *)
+let rec lemma_find_opt_parent_same_as_find_root (#n:nat) (uf:uf_forest n) (i:id n) (h:heap{live uf h /\ well_formed uf h}) (j:id n)
   :Lemma (requires True)
          (ensures  (let _, h0 = reify (find uf i h) h in
 	            let _, h1 = reify (find_opt uf i h) h in
 
-                    let p0, _ = reify (find uf j h0) h0 in
-		    let p1, _ = reify (find uf j h1) h1 in
-		    p0 = p1))
-	 (decreases (length uf - height uf j h))
-  = lemma_1 uf i h j;
+                    let p0 = parent uf j h0 in
+		    let p1 = parent uf j h1 in
+
+                    p0 = p1 \/ (p1 = fst (reify (find uf j h0) h0) /\ parent uf p1 h1 = p1)))
+	 (decreases (length uf - height #n uf i h))
+  = let p, _ = sel h (index uf i) in
+    if p = i then ()
+    else begin
+      lemma_find_opt_parent_same_as_find_root uf p h j;
+      ignore (reify (find uf p h) h);
+      ignore (reify (find_opt uf p h) h);
+      ignore (reify (find uf j h) h);  //AR: in general there is need for these triggers ... need to look into it
+      lemma_find_opt_helper uf i h;
+      if j <> i then ()
+      else begin  //else we invoke the lemma that find and find_opt return same result, for both p and i
+        lemma_find_find_opt_same_result uf i h;
+    	lemma_find_find_opt_same_result uf p h
+      end
+    end
+
+(*
+ * equivalence of find and find_opt
+ * in particular, we prove that find of a node j in h1 (the resultant heap after path compression)
+ * is same as find of j in h0
+ *)
+#set-options "--z3rlimit 50"
+let rec lemma_find_find_opt_equivalence (#n:nat) (uf:uf_forest n) (i:id n) (h:heap{live uf h /\ well_formed uf h}) (j:id n)
+  :Lemma (requires True)
+         (ensures  (let _, h0 = reify (find uf i h) h in
+	            let _, h1 = reify (find_opt uf i h) h in
+
+                    let r0, _ = reify (find uf j h0) h0 in
+		    let r1, _ = reify (find uf j h1) h1 in
+		    r0 = r1))  //root of a node remains same in h0 and h1, i.e. find_opt does not change the find query
+	 (decreases (length uf - height #n uf j h))
+  = 
     let _, h0 = reify (find uf i h) h in
     let _, h1 = reify (find_opt uf i h) h in
 
-    assert (h0 == h);
+    lemma_find_opt_parent_same_as_find_root uf i h j;
 
     let p0, _ = sel h0 (index uf j) in
     let p1, _ = sel h1 (index uf j) in
+    lemma_find_helper uf j h0;
+    lemma_find_helper uf j h1;
 
-    assert (p0 = p1 \/ (p1 = fst (reify (find uf j h) h) /\ parent uf p1 h1 = p1));
+    //lemma_find_opt_parent_same_as_find_root tells us that either p0 = p1,
+    //or p1 = root of j in h0
+  
     if p0 = p1 then begin
-      assert (forall (i:id uf). height uf i h < length uf);
-      assume (height uf p0 h > height uf j h);
-      lemma_2 uf i h p0;
-      () //this actually goes through, takes time
+      if j = p0 then ()  //if j = p0 = p1, then find returns j immediately, so we are done
+      else begin  //else we invoke I.H. on p0, and then one unrolling of find call on j uses it to give us the proof
+        lemma_find_find_opt_equivalence uf i h p0
+      end
     end
-    else begin
-      assert (p1 = fst (reify (find uf j h) h));
-      if (p1 = j) then ()
-      else
-        assert (fst (reify (find uf j h1) h1) = fst (reify (find uf p1 h1) h1));
+    else  //p0 <> p1, but p1 = root of j in h0 and p1's parent = p1 in h1, so, root of j in h1 is p1 = root of j in h0
+      begin
+        assert (p1 = fst (reify (find uf j h0) h0));
 	assert (parent uf p1 h1 = p1);
-	assert (fst (reify (find uf p1 h1) h1) = p1);
+	assert (p1 = fst (reify (find uf p1 h1) h1));
 	()
-    end
-      
-	(* assert (forall (i:id uf). let j = parent uf i h in *)
-	(*                      j <> r_1 ==> addr_of (index uf j) <> addr_of ref_1); *)
-	(* assert (forall (i:id uf). ~ (parent uf i h = r_1 \/ parent uf i h = r_2) ==>  *)
-	(*                      (addr_of (index uf i) <> addr_of ref_1 /\ *)
-	(* 		      addr_of (index uf i) <> addr_of ref_2 /\ *)
-	(* 		      addr_of (index uf (parent uf i h)) <> addr_of ref_1 /\ *)
-	(* 		      addr_of (index uf (parent uf i h)) <> addr_of ref_2)); *)
-        //assert (forall (i:id uf). ~ (parent uf i h = r_2 \/ parent uf i h = r_1 \/ parent uf i h = i) ==> height uf i h < height uf (parent uf i h) h);
-	//assert (well_formed uf h);
-
-
-    //let h0 = STATE?.get () in
-    //assert (well_formed uf h0);
-    //assert (forall (i:id uf). ~ (parent uf i h0 = r_2 \/ parent uf i h0 = r_1 \/ parent uf i h0 = i) ==> height uf i h0 < height uf (parent uf i h0) h0);
-    //assert (forall (i:id uf). ~ (parent uf i h0 = r_2 \/ parent uf i h0 = r_1) ==> height uf i h0 < height uf (parent uf i h0) h0);
-    (* assert (forall (i:id uf). (parent uf i h0 = r_2 /\ addr_of (index uf i) <> addr_of ref_2) ==> height uf i h0 < height uf (parent uf i h0) h0); *)
-    (* admit () *)
-
-      
-      
-      (* let h0' = STATE?.get () in *)
-      (* let _ = write ref_1 (p_2, d_2 + 1) in () in *)
-      (* let h1 = STATE?.get () in *)
-      (* assert (forall (i:id uf). parent uf i h1 < length uf); *)
-      (* assert (live uf h1); *)
-      (* assert (forall (i:id uf). i <> r_1 ==> addr_of (index uf i) <> addr_of (index uf r_1)); *)
-      (* assert (forall (a:Type) (r:ref a). addr_of r <> addr_of ref_1 ==> sel h1 r == sel h0' r); *)
-      (* assert (forall (i:id uf). (i <> r_1) ==> addr_of (index uf i) <> addr_of ref_1); *)
-      (* assert (forall (i:id uf). (i <> r_1 ==> sel h1 (index uf i) = sel h0' (index uf i))); *)
-      (* assert (forall (i:id uf). (i <>r_1 ==> (parent uf i h1 = i \/ depth uf i h1 > depth uf (parent uf i h1) h1))); *)
-      (* admit () *)
-  
-  
-  (* let r_1 = index uf i_1 in *)
-  (*   let r_2 = index uf i_2 in *)
-  
-  (*   let p_1, d_1 = read r_1 in *)
-  (*   let p_2, d_2 = read r_2 in *)
-  
-  (*   if p_1 = p_2 then () *)
-  (*   else *)
-  (*     write r_1 (p_2, d_2 +      *)
-
-        (* let h = STATE?.get () in *)
-	(* assert (forall (i:id uf). parent uf i h < length uf); *)
-	(* assert (forall (i:id uf). height uf i h < length uf); *)
-	(* assert (height uf r_1 h < height uf (parent uf r_1 h) h); *)
-	(* assert (parent uf r_2 h = r_2); *)
-	
-	(* assert (forall (i:id uf). (addr_of (index uf i) <> addr_of ref_1 /\ *)
-	(*                       addr_of (index uf i) <> addr_of ref_2) ==> sel h (index uf i) = sel h0 (index uf i)); *)
-        (* assert (forall (i:id uf). parent uf i h = r_1 ==> height uf i h < height uf (parent uf i h) h); *)
-        (* assert (forall (i:id uf). (parent uf i h = r_2 ==> (i = r_2 \/ height uf i h < height uf (parent uf i h) h))); *)
-	(* //assert (live uf h); *)
-	(* assert (index uf r_1 == ref_1); *)
+      end
